Moved sync out of phaser.

src/Phasers/Phaser.v
@@ -196,54 +196,6 @@ Section Defs.
   Defined.
 
   (**
-    Predicate [Sync] defines what happens when a
-    task synchronizes with the other members of a phaser, which is triggered when
-    a task performs either wait on a phaser, or next.
-    The semantics of [Sync] depends on the registration mode of the task.
-    Tasks registered in [SIGNAL_ONLY] mode do not block, so predicate [Sync] always
-    holds. Tasks that are not registered in [SIGNAL_ONLY] mode
-    (that is tasks with a wait capability) only holds once all 
-    members with a signal capability issued at least as many signals as the task
-    synchronizing.
-   *)
-
-  Inductive Sync : phaser -> tid -> Prop :=
-  | sync_def:
-    forall ph t v,
-    MapsTo t v ph ->
-    CanWait (mode v) ->
-    Phase ph (S (wait_phase v)) ->
-    Sync ph t.
-
-  Definition sync x ph:
-    { Sync ph x } + { ~ Sync ph x }.
-  Proof.
-    intros.
-    remember (find x ph).
-    symmetry in Heqo.
-    destruct o as [v|]. {
-      rewrite <- Map_TID_Facts.find_mapsto_iff in *.
-      destruct (can_wait_so (mode v)). {
-        destruct (phase ph (S (wait_phase v))). {
-          eauto using sync_def.
-        }
-        right; unfold not; intros N; inversion N; subst; clear N;
-        assert (v0 = v) by eauto using Map_TID_Facts.MapsTo_fun; subst.
-        contradiction.
-      }
-      right; unfold not; intros N; inversion N; subst; clear N;
-      assert (v0 = v) by eauto using Map_TID_Facts.MapsTo_fun; subst.
-      rewrite e in *.
-      inversion H0.
-    }
-    right; unfold not; intros N.
-    inversion N; subst; clear N;
-    rewrite Map_TID_Facts.find_mapsto_iff in *;
-    rewrite H in *;
-    inversion Heqo.
-  Defined.
-
-  (**
     Wait consists of thee pre-conditions: (i) task [t] is registered in phaser [ph],
     (ii) task [t] has signalled as per [Taskview.WaitPre],
     and (iii) task [t] must be able to synchronize with the other members through phaser [ph].
@@ -254,7 +206,7 @@ Section Defs.
       forall v,
       Map_TID.MapsTo t v ph ->
       Taskview.WaitPre v ->
-      Sync ph t ->
+      Phase ph (S (wait_phase v)) ->
       WaitPre t ph.
 
   Definition wait_pre x ph:
@@ -265,15 +217,20 @@ Section Defs.
     destruct o as [v|]. {
       rewrite <- Map_TID_Facts.find_mapsto_iff in *.
       destruct (Taskview.wait_pre v). {
-        destruct (sync x ph). {
+        destruct (phase ph (S (wait_phase v))). {
           eauto using wait_pre_def.
         }
-        right; unfold not; intros N;
-        inversion N; contradiction.
+        right.
+        unfold not; intros N.
+        destruct N.
+        assert (v0 = v) by eauto using  Map_TID_Facts.MapsTo_fun; subst.
+        contradiction n.
       }
-      right; unfold not; intros N.
-      inversion N;
-      assert (v0 = v) by eauto using Map_TID_Facts.MapsTo_fun; subst; contradiction.
+      right.
+      unfold not; intros N.
+      destruct N.
+      assert (v0 = v) by eauto using  Map_TID_Facts.MapsTo_fun; subst.
+      contradiction n.
     }
     right; unfold not; intros N.
     inversion N.
