src/Phasers/PhaseOrdering/Phaser.v
@@ -217,14 +217,13 @@ Section Facts.
             inversion H1; simpl in *; subst; clear H1.
             inversion H3; simpl in *; subst; clear H3.
             inversion H7; subst; clear H7.
-            assert (v0 = v) by eauto using Map_TID_Facts.MapsTo_fun; subst.
             inversion H8; subst; clear H8.
-            assert (v0 = v) by eauto using Map_TID_Facts.MapsTo_fun; subst.
+            simpl_red.
+            rename v0 into v2.
             destruct (Regmode.can_signal_wo (mode v1)). {
               apply tv_nhb_ge.
-              assert (signal_phase v1 >= S (wait_phase v)) by (inversion H11; eauto).
               rewrite wait_wait_phase.
-              intuition.
+              eauto.
             }
             auto using tv_nhb_wo.
           - apply tv_nhb_so.
@@ -826,11 +825,9 @@ Section Facts.
     - subst.
       assert (v' = v) by eauto using Map_TID_Facts.MapsTo_fun; subst; clear H6.
       assert (Taskview.Facilitates v1 v) by eauto using well_ordered_to_facilitates.
-      inversion H3; subst.
-      assert (v0 = v) by eauto using Map_TID_Facts.MapsTo_fun; subst; clear H5.
-      inversion H7.
-      assert (Hx := H5 _ _ H0); clear H5 H7.
-      apply wait_preserves_rhs; auto.
+      rename v into v2.
+      destruct H3.
+      apply wait_preserves_rhs; eauto.
     - eauto using well_ordered_to_facilitates.
   Qed.
 
